combine files

Cslib/Languages/LambdaCalculus/LocallyNameless/Fsub/Opening.lean
@@ -10,7 +10,7 @@ import Cslib.Languages.LambdaCalculus.LocallyNameless.Fsub.Basic
 /-! # λ-calculus
 
 The λ-calculus with polymorphism and subtyping, with a locally nameless representation of syntax.
-This file defines opening and local closure.
+This file defines opening, local closure, and substitution.
 
 ## References
 
@@ -22,7 +22,7 @@ This file defines opening and local closure.
 
 universe u
 
-variable {Var : Type u}
+variable {Var : Type u} [HasFresh Var] [DecidableEq Var]
 
 namespace LambdaCalculus.LocallyNameless.Fsub
 
@@ -39,11 +39,6 @@ def openRec (X : ℕ) (δ : Ty Var) : Ty Var → Ty Var
 | sum σ τ => sum (openRec X δ σ) (openRec X δ τ)
 
 scoped notation:68 γ "⟦" X " ↝ " δ "⟧ᵞ"=> openRec X δ γ
-
-/-- An opening appearing in both sides of an equality of types can be removed. -/
-@[scoped grind]
-lemma openRec_neq_eq {σ τ γ : Ty Var} (neq : X ≠ Y) (h : σ⟦Y ↝ τ⟧ᵞ = σ⟦Y ↝ τ⟧ᵞ⟦X ↝ γ⟧ᵞ) : 
-    σ = σ⟦X ↝ γ⟧ᵞ := by induction σ generalizing Y X <;> grind
 
 /-- Variable opening (type opening to type) of the closest binding. -/
 @[scoped grind =]
@@ -62,12 +57,74 @@ inductive LC : Ty Var → Prop
 
 attribute [scoped grind] LC.top LC.var LC.arrow LC.sum
 
-variable [HasFresh Var] [DecidableEq Var]
+/-- Type substitution. -/
+@[scoped grind =]
+def subst (X : Var) (δ : Ty Var) : Ty Var → Ty Var
+| top => top
+| bvar J => bvar J
+| fvar Y => if Y = X then δ else fvar Y
+| arrow σ τ => arrow (subst X δ σ) (subst X δ τ)
+| all σ τ => all (subst X δ σ) (subst X δ τ)
+| sum σ τ => sum (subst X δ σ) (subst X δ τ)
+
+instance : HasSubstitution (Ty Var) Var (Ty Var) where
+  subst γ X δ := Ty.subst X δ γ
+
+variable {σ τ δ γ : Ty Var}
+
+omit [HasFresh Var] [DecidableEq Var] in
+/-- An opening appearing in both sides of an equality of types can be removed. -/
+@[scoped grind]
+lemma openRec_neq_eq {σ τ γ : Ty Var} (neq : X ≠ Y) (h : σ⟦Y ↝ τ⟧ᵞ = σ⟦Y ↝ τ⟧ᵞ⟦X ↝ γ⟧ᵞ) : 
+    σ = σ⟦X ↝ γ⟧ᵞ := by induction σ generalizing Y X <;> grind
 
 /-- A locally closed type is unchanged by opening. -/
 @[scoped grind =_]
 lemma openRec_lc {σ τ : Ty Var} (lc : σ.LC) : σ = σ⟦X ↝ τ⟧ᵞ := by
   induction lc generalizing X <;> (have := fresh_exists <| free_union Var; grind)
+
+omit [HasFresh Var] in
+@[scoped grind _=_]
+lemma subst_def : Ty.subst (X : Var) (δ : Ty Var) (γ : Ty Var) = γ[X := δ] := by rfl
+
+omit [HasFresh Var] in
+/-- Substitution of a free variable not present in a type leaves it unchanged. -/
+@[scoped grind <=]
+lemma subst_fresh (nmem : X ∉ γ.fv) (δ : Ty Var) : γ = γ[X := δ] := by
+  induction γ <;> grind
+
+/-- Substitution of a locally closed type distributes with opening. -/
+@[scoped grind]
+lemma openRec_subst (Y : ℕ) (σ τ : Ty Var) (lc : δ.LC) (X : Var) : 
+    (σ⟦Y ↝ τ⟧ᵞ)[X := δ] = σ[X := δ]⟦Y ↝ τ[X := δ]⟧ᵞ := by
+  induction σ generalizing Y
+  all_goals grind
+
+/-- Specialize `Ty.openRec_subst` to the first opening. -/
+lemma open_subst (σ τ : Ty Var) (lc : δ.LC) (X : Var) : (σ ^ᵞ τ)[X := δ] = σ[X := δ] ^ᵞ τ[X := δ]
+  := openRec_subst 0 σ τ lc X
+
+/-- Specialize `Ty.subst_open` to free variables. -/
+lemma open_subst_var (σ : Ty Var) (neq : Y ≠ X) (lc : δ.LC) :
+    (σ ^ᵞ fvar Y)[X := δ] = (σ[X := δ]) ^ᵞ fvar Y := by grind [open_subst]
+
+omit [HasFresh Var] in
+/-- Opening to a type is equivalent to opening to a free variable and substituting. -/
+@[scoped grind]
+lemma openRec_subst_intro (Y : ℕ) (δ : Ty Var) (nmem : X ∉ γ.fv) :
+    γ⟦Y ↝ δ⟧ᵞ = (γ⟦Y ↝ fvar X⟧ᵞ)[X := δ] := by
+  induction γ generalizing δ Y <;> grind
+
+omit [HasFresh Var] in
+/-- Specialize `Ty.openRec_subst_intro` to the first opening. -/
+lemma open_subst_intro (δ : Ty Var) (nmem : X ∉ γ.fv) : γ ^ᵞ δ = (γ ^ᵞ fvar X)[X := δ] := 
+  openRec_subst_intro _ _ nmem
+
+@[scoped grind =>]
+lemma subst_lc (σ_lc : σ.LC) (τ_lc : τ.LC) (X : Var) : σ[X := τ].LC := by
+  induction σ_lc
+  case all => apply LC.all (free_union Var) <;> grind
+  all_goals grind 
 
 end Ty
 
@@ -91,12 +148,6 @@ def openRec_ty (X : ℕ) (δ : Ty Var) : Term Var → Term Var
 
 scoped notation:68 t "⟦" X " ↝ " δ "⟧ᵗᵞ"=> openRec_ty X δ t
 
-/-- An opening (term to type) appearing in both sides of an equality of terms can be removed. -/
-@[scoped grind]
-lemma openRec_ty_neq_eq (neq : X ≠ Y) (eq : t⟦Y ↝ σ⟧ᵗᵞ = t⟦Y ↝ σ⟧ᵗᵞ⟦X ↝ τ⟧ᵗᵞ) : 
-    t = t⟦X ↝ τ⟧ᵗᵞ := by
-  induction t generalizing X Y <;> grind
-
 /-- Variable opening (term opening to type) of the closest binding. -/
 @[scoped grind =]
 def open_ty (t : Term Var) (δ : Ty Var) := openRec_ty 0 δ t
@@ -118,12 +169,6 @@ def openRec_tm (x : ℕ) (s : Term Var) : Term Var → Term Var
 | case t₁ t₂ t₃ => case (openRec_tm x s t₁) (openRec_tm (x + 1) s t₂) (openRec_tm (x + 1) s t₃)
 
 scoped notation:68 t "⟦" x " ↝ " s "⟧ᵗᵗ"=> openRec_tm x s t
-
-/-- An opening (term to term) appearing in both sides of an equality of terms can be removed. -/
-@[scoped grind]
-lemma openRec_tm_neq_eq (neq : x ≠ y) (eq : t⟦y ↝ s₁⟧ᵗᵗ = t⟦y ↝ s₁⟧ᵗᵗ⟦x ↝ s₂⟧ᵗᵗ) : 
-    t = t⟦x ↝ s₂⟧ᵗᵗ := by
-  induction t generalizing x y <;> grind
 
 /-- Variable opening (term opening to term) of the closest binding. -/
 @[scoped grind =]
@@ -150,19 +195,20 @@ inductive LC : Term Var → Prop
 
 attribute [scoped grind] LC.var LC.app LC.inl LC.inr LC.tapp
 
-variable {t s : Term Var} {x y X Y : ℕ} {σ δ : Ty Var}
+variable {t : Term Var} {δ : Ty Var}
 
+omit [HasFresh Var] [DecidableEq Var] in
+/-- An opening (term to type) appearing in both sides of an equality of terms can be removed. -/
+@[scoped grind]
+lemma openRec_ty_neq_eq (neq : X ≠ Y) (eq : t⟦Y ↝ σ⟧ᵗᵞ = t⟦Y ↝ σ⟧ᵗᵞ⟦X ↝ τ⟧ᵗᵞ) : 
+    t = t⟦X ↝ τ⟧ᵗᵞ := by
+  induction t generalizing X Y <;> grind
+
+omit [HasFresh Var] [DecidableEq Var] in
 /-- Elimination of mixed term and type opening. -/
 @[scoped grind]
 lemma openRec_tm_ty_eq (eq : t⟦x ↝ s⟧ᵗᵗ = t⟦x ↝ s⟧ᵗᵗ⟦y ↝ δ⟧ᵗᵞ) : t = t⟦y ↝ δ⟧ᵗᵞ
   := by induction t generalizing x y <;> grind
-
-/-- Elimination of mixed term and type opening. -/
-@[scoped grind]
-lemma openRec_ty_tm_eq (eq : t⟦Y ↝ σ⟧ᵗᵞ = t⟦Y ↝ σ⟧ᵗᵞ⟦x ↝ s⟧ᵗᵗ) : t = t⟦x ↝ s⟧ᵗᵗ := by
-  induction t generalizing x Y <;> grind
-
-variable [HasFresh Var] [DecidableEq Var]
 
 /-- A locally closed term is unchanged by type opening. -/
 @[scoped grind]
@@ -178,6 +224,170 @@ lemma openRec_tm_lc (lc : t.LC) : t = t⟦x ↝ s⟧ᵗᵗ := by
   case abs  | tabs | let' | case => sorry
   all_goals grind
 
+/-- Substitution of a type within a term. -/
+@[scoped grind =]
+def subst_ty (X : Var) (δ : Ty Var) : Term Var → Term Var
+| bvar x => bvar x
+| fvar x => fvar x
+| abs σ t₁ => abs (σ [X := δ]) (subst_ty X δ t₁)
+| app t₁ t₂ => app (subst_ty X δ t₁) (subst_ty X δ t₂)
+| tabs σ t₁ => tabs (σ [X := δ]) (subst_ty X δ t₁)
+| tapp t₁ σ => tapp (subst_ty X δ t₁) (σ[X := δ])
+| let' t₁ t₂ => let' (subst_ty X δ t₁) (subst_ty X δ t₂)
+| inl t₁ => inl (subst_ty X δ t₁)
+| inr t₁ => inr (subst_ty X δ t₁)
+| case t₁ t₂ t₃ => case (subst_ty X δ t₁) (subst_ty X δ t₂) (subst_ty X δ t₃)
+
+instance : HasSubstitution (Term Var) Var (Ty Var) where
+  subst t X δ := Term.subst_ty X δ t
+
+omit [HasFresh Var] in
+@[scoped grind _=_]
+lemma subst_ty_def : subst_ty (X : Var) (δ : Ty Var) (t : Term Var) = t[X := δ] := by rfl
+
+omit [HasFresh Var] in
+/-- Substitution of a free type variable not present in a term leaves it unchanged. -/
+lemma subst_ty_fresh (nmem : X ∉ t.fv_ty) (δ : Ty Var) : t = t [X := δ] := 
+  by induction t <;> grind
+
+/-- Substitution of a locally closed type distributes with term opening to a type . -/
+@[scoped grind]
+lemma openRec_ty_subst_ty (Y : ℕ) (t : Term Var) (σ : Ty Var) (lc : δ.LC) (X : Var) : 
+    (t⟦Y ↝ σ⟧ᵗᵞ)[X := δ] = (t[X := δ])⟦Y ↝  σ[X := δ]⟧ᵗᵞ := by
+  induction t generalizing Y <;> grind
+
+/-- Specialize `Term.openRec_ty_subst` to the first opening. -/
+lemma open_ty_subst_ty (t : Term Var) (σ : Ty Var) (lc : δ.LC) (X : Var) :
+     (t ^ᵗᵞ σ)[X := δ] = t[X := δ] ^ᵗᵞ σ[X := δ] := openRec_ty_subst_ty 0 t σ lc X
+
+/-- Specialize `Term.open_ty_subst` to free type variables. -/
+lemma open_ty_subst_ty_var (t : Term Var) (neq : Y ≠ X) (lc : δ.LC) :
+    (t ^ᵗᵞ .fvar Y)[X := δ] = t[X := δ] ^ᵗᵞ .fvar Y := by grind
+
+omit [HasFresh Var]
+
+/-- Opening a term to a type is equivalent to opening to a free variable and substituting. -/
+lemma openRec_ty_subst_ty_intro (Y : ℕ) (t : Term Var) (nmem : X ∉ t.fv_ty) : 
+  t⟦Y ↝ δ⟧ᵗᵞ = (t⟦Y ↝ Ty.fvar X⟧ᵗᵞ)[X := δ] := by
+  induction t generalizing X δ Y <;> grind
+
+/-- Specialize `Term.openRec_ty_subst_ty_intro` to the first opening. -/
+lemma open_ty_subst_ty_intro (t : Term Var) (δ : Ty Var) (nmem : X ∉ t.fv_ty) : 
+    t ^ᵗᵞ δ = (t ^ᵗᵞ Ty.fvar X)[X := δ] := openRec_ty_subst_ty_intro _ _ nmem
+
+/-- Substitution of a term within a term. -/
+@[scoped grind =]
+def subst_tm (x : Var) (s : Term Var) : Term Var → Term Var
+| bvar x => bvar x
+| fvar y => if y = x then s else fvar y
+| abs σ t₁ => abs σ (subst_tm x s t₁)
+| app t₁ t₂ => app (subst_tm x s t₁) (subst_tm x s t₂)
+| tabs σ t₁ => tabs σ (subst_tm x s t₁)
+| tapp t₁ σ => tapp (subst_tm x s t₁) σ
+| let' t₁ t₂ => let' (subst_tm x s t₁) (subst_tm x s t₂)
+| inl t₁ => inl (subst_tm x s t₁)
+| inr t₁ => inr (subst_tm x s t₁)
+| case t₁ t₂ t₃ => case (subst_tm x s t₁) (subst_tm x s t₂) (subst_tm x s t₃)
+
+instance : HasSubstitution (Term Var) Var (Term Var) where
+  subst t x s := Term.subst_tm x s t
+
+@[scoped grind _=_]
+lemma subst_tm_def : subst_tm (x : Var) (s : Term Var) (t : Term Var) = t[x := s] := by rfl
+
+variable {t s : Term Var} {δ : Ty Var} {x : Var}
+
+/-- Substitution of a free term variable not present in a term leaves it unchanged. -/
+lemma subst_tm_fresh (nmem : x ∉ t.fv_tm) (s : Term Var) : t = t[x := s] := by
+  induction t <;> grind
+
+variable [HasFresh Var]
+
+/-- Substitution of a locally closed term distributes with term opening to a term. -/
+lemma openRec_tm_subst_tm (y : ℕ) (t₁ t₂ : Term Var) (lc : s.LC) (x : Var) :
+    (t₁⟦y ↝ t₂⟧ᵗᵗ)[x := s] = (t₁[x := s])⟦y ↝  t₂[x := s]⟧ᵗᵗ := by
+  induction t₁ generalizing y <;> grind
+
+/-- Specialize `Term.openRec_tm_subst_tm` to the first opening. -/
+lemma open_tm_subst_tm (t₁ t₂ : Term Var) (lc : s.LC) (x : Var) :
+    (t₁ ^ᵗᵗ t₂)[x := s] = (t₁[x := s]) ^ᵗᵗ t₂[x := s] := openRec_tm_subst_tm 0 t₁ t₂ lc x
+
+/-- Specialize `Term.openRec_tm_subst_tm` to free term variables. -/ 
+lemma open_tm_subst_tm_var (t : Term Var) (neq : y ≠ x) (lc : s.LC) :
+     (t ^ᵗᵗ fvar y)[x := s] = (t[x := s]) ^ᵗᵗ fvar y := by grind [open_tm_subst_tm]
+
+/-- Substitution of a locally closed type distributes with term opening to a term. -/
+lemma openRec_tm_subst_ty (y : ℕ) (t₁ t₂ : Term Var) (δ : Ty Var) (X : Var) :
+    (t₁⟦y ↝ t₂⟧ᵗᵗ)[X := δ] = (t₁[X := δ])⟦y ↝  t₂[X := δ]⟧ᵗᵗ := by
+  induction t₁ generalizing y <;> grind
+
+/-- Specialize `Term.openRec_tm_subst_ty` to the first opening -/
+lemma open_tm_subst_ty (t₁ t₂ : Term Var) (δ : Ty Var) (X : Var) :
+    (t₁ ^ᵗᵗ t₂)[X := δ] = (t₁[X := δ]) ^ᵗᵗ t₂[X := δ] := openRec_tm_subst_ty 0 t₁ t₂ δ X
+
+/-- Specialize `Term.open_tm_subst_ty` to free term variables -/
+lemma open_tm_subst_ty_var (t₁ : Term Var) (δ : Ty Var) (X y : Var) :
+    (t₁ ^ᵗᵗ fvar y)[X := δ] = (t₁[X := δ]) ^ᵗᵗ fvar y := by grind [open_tm_subst_ty]
+
+/-- Substitution of a locally closed term distributes with term opening to a type. -/
+lemma openRec_ty_subst_tm (Y : ℕ) (t : Term Var) (δ : Ty Var) (lc : s.LC) (x : Var) :
+    (t⟦Y ↝ δ⟧ᵗᵞ)[x := s] = t[x := s]⟦Y ↝ δ⟧ᵗᵞ := by
+  induction t generalizing Y <;> grind
+
+/-- Specialize `Term.openRec_ty_subst_tm` to the first opening. -/
+lemma open_ty_subst_tm (t : Term Var) (δ : Ty Var) (lc : s.LC) (x : Var) :
+    (t ^ᵗᵞ δ)[x := s] = t[x := s] ^ᵗᵞ δ := openRec_ty_subst_tm 0 t δ lc x
+
+/-- Specialize `Term.open_ty_subst_tm` to free type variables. -/
+lemma open_ty_subst_tm_var (t : Term Var) (lc : s.LC) (x Y : Var) :
+    (t ^ᵗᵞ .fvar Y)[x := s] = t[x := s] ^ᵗᵞ .fvar Y := open_ty_subst_tm _ _ lc _
+
+omit [HasFresh Var]
+
+/-- Opening a term to a term is equivalent to opening to a free variable and substituting. -/
+lemma openRec_tm_subst_tm_intro (y : ℕ) (t s : Term Var) (nmem : x ∉ t.fv_tm) :
+    t⟦y ↝ s⟧ᵗᵗ = (t⟦y ↝ fvar x⟧ᵗᵗ)[x := s] := by
+  induction t generalizing y <;> grind
+
+/-- Specialize `Term.openRec_tm_subst_tm_intro` to the first opening. -/
+lemma open_tm_subst_tm_intro (t s : Term Var) (nmem : x ∉ t.fv_tm) :
+    t ^ᵗᵗs = (t ^ᵗᵗ fvar x)[x := s] := openRec_tm_subst_tm_intro _ _ _ nmem
+
+variable [HasFresh Var]
+
+lemma subst_ty_lc (t_lc : t.LC) (δ_lc : δ.LC) (X : Var) : t[X := δ].LC := by
+  induction t_lc
+  case abs | tabs | let' | case => sorry
+  all_goals grind
+
+lemma subst_tm_lc (t_lc : t.LC) (s_lc : s.LC) (x : Var) : t[x := s].LC := by
+  induction t_lc
+  case abs | tabs | let' | case => sorry
+  all_goals grind
+
 end Term
+
+namespace Binding
+
+omit [HasFresh Var]
+
+/-- Binding substitution of types. -/
+@[scoped grind =]
+def subst (X : Var) (δ : Ty Var) : Binding Var → Binding Var
+| sub γ => sub <| γ[X := δ]
+| ty  γ => ty  <| γ[X := δ]
+
+instance : HasSubstitution (Binding Var) Var (Ty Var) where
+  subst γ X δ := Binding.subst X δ γ
+
+variable {δ γ : Ty Var} {X : Var}
+
+@[scoped grind _=_]
+lemma subst_sub : (sub γ)[X := δ] = sub (γ[X := δ]) := by rfl
+
+@[scoped grind _=_]
+lemma subst_ty : (ty γ)[X := δ] = ty (γ[X := δ]) := by rfl
+
+end Binding
 
 end LambdaCalculus.LocallyNameless.Fsub
